Add basic quickCode support for lemma calls, assert, assume, old

tools/Vale/src/emit_common_quick_code.fs
@@ -11,27 +11,48 @@ open Emit_common_base
 open Microsoft.FSharp.Math
 open System.Numerics
 
-let rec build_qcode_stmt (s:stmt):exp =
+let rec build_qcode_stmt (env:env) (s:stmt) ((needsState:bool), (eTail:exp)):(bool * exp) =
   let err () = internalErr "make_gen_quick_block" in
   match skip_loc_stmt s with
   | SAssign ([], e) ->
     (
       match skip_loc e with
-      | EApply(Id x, es) ->
-          let es = List.filter (fun e -> match e with EOp (Uop UGhostOnly, _) -> false | _ -> true) es in
-          let es = List.map get_code_exp es in
+      | EApply (Id x, es) when Map.containsKey (Id x) env.procs ->
+          let es = List.map get_lemma_exp es in
           let es = List.map (map_exp stateToOp) es in
           let es = List.map exp_refined es in
-          vaApp ("quick_" + x) es
+          let e = vaApp ("quick_" + x) es in
+          if needsState then
+            let fTail = EBind (Lambda, [], [(Reserved "s", Some tState); (Id "_", None)], [], eTail) in
+            (false, EApply (Id "QBind", [e; fTail]))
+          else
+            (false, EApply (Id "QSeq", [e; eTail]))
+      | EApply (x, es) ->
+          let es = List.map get_lemma_exp es in
+          let es = List.map (map_exp stateToOp) es in
+          let es = List.map exp_refined es in
+          let eApp = EApply (x, es) in
+          let fApp = EBind (Lambda, [], [(Id "_", Some tUnit)], [], eApp) in
+          (true, EApply (Id "wpLemma", [fApp; eTail]))
       | _ -> err ()
     )
+  | SAssume e ->
+      let sAssign = SAssign ([], EApply (Reserved "assume", [e])) in
+      build_qcode_stmt env sAssign (needsState, eTail)
+  | SAssert (_, e) ->
+      let sAssign = SAssign ([], EApply (Reserved "assert", [e])) in
+      build_qcode_stmt env sAssign (needsState, eTail)
   | _ -> err ()
-and build_qcode_stmts (ss:stmt list):exp =
+and build_qcode_stmts (env:env) (ss:stmt list):exp =
   let empty = EApply (Id "QEmpty", []) in
-  let cons el e = EApply (Id "QSeq", [e; el]) in
-  List.fold cons empty (List.rev (List.map build_qcode_stmt ss))
-and build_qcode_block (ss:stmt list):exp =
-  EApply (Id "qblock", [build_qcode_stmts ss])
+  let (needsState, e) = List.foldBack (build_qcode_stmt env) ss (false, empty) in
+  e
+and build_qcode_block (add_old:bool) (env:env) (ss:stmt list):exp =
+  let s = Reserved "s" in
+  let eStmts = build_qcode_stmts env ss in
+  let eLet = if add_old then EBind (BindLet, [EVar s], [(Reserved "old_s", Some tState)], [], eStmts) else eStmts in
+  let fApp = EBind (Lambda, [], [(s, Some tState)], [], eLet) in
+  EApply (Id "qblock", [fApp])
 
 let make_gen_quick_block (loc:loc) (p:proc_decl):((env -> quick_info -> lhs list -> exp list -> stmt list -> stmt list) * (unit -> decls)) =
   let funs = ref ([]:decls) in
@@ -42,15 +63,15 @@ let make_gen_quick_block (loc:loc) (p:proc_decl):((env -> quick_info -> lhs list
     let cid = Reserved ("code_" + info.qsym + "_" + (string_of_id p.pname)) in
     let tArgs = List.map (fun (x, _) -> TName x) fParams in
     let tCodeApp = TApp (TName cid, tArgs) in
-//    let fBody = build_qcode_block ss in
-    let fBody = build_qcode_stmts ss in
+//    let fBody = build_qcode_block false env ss in
+    let fBody = build_qcode_stmts env ss in
     let fCode =
       {
         fname = id;
         fghost = Ghost;
         fargs = fParams;
-//        fret = TApp (TName (Reserved "quickCode"), [TName (Id "unit"); tCodeApp]);
-        fret = TApp (TName (Id "quickCodes"), [TName (Id "unit"); tCodeApp]);
+//        fret = TApp (TName (Reserved "quickCode"), [tUnit; tCodeApp]);
+        fret = TApp (TName (Id "quickCodes"), [tUnit; tCodeApp]);
         fbody = Some fBody;
         fattrs = [(Id "opaque_to_smt", [])];
       }
@@ -91,6 +112,7 @@ let build_qcode (env:env) (loc:loc) (p:proc_decl) (ss:stmt list):decls =
   (*
   [@"opaque_to_smt"]
   let va_qcode_Add3 () : quickCode unit (va_code_Add3 ()) = qblock (
+    fun (va_s:state) -> let va_old_s = va_s in
     QSeq (va_quick_Add64 (OReg Rax) (OConst 1)) (
     QSeq (va_quick_Add64 (OReg Rax) (OConst 1)) (
     QSeq (va_quick_Add64 (OReg Rax) (OConst 1)) (
@@ -102,8 +124,8 @@ let build_qcode (env:env) (loc:loc) (p:proc_decl) (ss:stmt list):decls =
   let cid = Reserved ("code_" + (string_of_id p.pname)) in
   let tArgs = List.map (fun (x, _) -> TName x) fParams in
   let tCodeApp = TApp (TName cid, tArgs) in
-  let tRetQuick = TApp (TName (Id "quickCode"), [TName (Id "unit"); tCodeApp]) in
-  let eQuick = build_qcode_block ss in
+  let tRetQuick = TApp (TName (Id "quickCode"), [tUnit; tCodeApp]) in
+  let eQuick = build_qcode_block true env ss in
   let fCodes =
     {
       fname = Reserved ("qcode_" + (string_of_id p.pname));
